Bytes.fst version 0.1

ulib/FStar.Bytes.fst
@@ -1,19 +1,282 @@
 module FStar.Bytes
-type byte = FStar.UInt8.byte
 
-open FStar.All
+open FStar.Seq
 
-assume type bytes
-assume HasEq_bytes: hasEq bytes
+module U = FStar.UInt
+module U8 = FStar.UInt8
+module U16 = FStar.UInt16
+module U32 = FStar.UInt32
+module U64 = FStar.UInt64
 
-assume val length : bytes -> Tot nat
-assume val get : b:bytes -> pos:nat{pos < length b} -> Tot byte
-assume val make : f:(nat -> Tot byte) -> len:nat -> Tot (b:bytes{length b = len})
-assume val zero_create : n:nat -> Tot (b:bytes{length b = n})
-assume val sub : b:bytes -> s:nat{s < length b} -> e:nat{e < length b /\ s <= e} -> Tot (sub:bytes{length sub = e - s + 1})
-assume val set : b:bytes -> n:nat{n < length b} -> byte -> unit
-assume val string_as_unicode_bytes : string -> bytes
-assume val utf8_bytes_as_string : bytes -> string
-assume val unicode_bytes_as_string : bytes -> string
-assume val string_as_utf8_bytes : string -> bytes
-assume val append : bytes -> bytes -> bytes
+type byte = U8.t
+abstract type bytes = seq byte
+abstract type string = seq FStar.Char.char
+
+let length (b:bytes) : Tot (n:nat{n = Seq.length b}) = Seq.length b
+
+val index: b:bytes -> i:nat{i < length b} -> Tot byte
+let index b i = Seq.index b i
+
+(*
+abstract val createEmpty: #a:Type -> Tot (s:(seq a){length s=0})
+let createEmpty #a = MkSeq []
+*)
+
+//val createEmpty: Tot (s:(bytes){length s=0})
+
+val create: len:nat -> v:byte -> Tot (bytes)
+let rec create len v =
+  if len = 0 then Seq.createEmpty
+  else cons v (create (len - 1) v)
+
+val init: len:nat -> contents: (i:nat { i < len } -> Tot byte) -> Tot (bytes)
+let rec init_aux (len:nat) (k:nat{k < len}) (contents:(i:nat { i < len } -> Tot byte))
+  : Tot (bytes) (decreases (len - k)) =
+  if k + 1 = len then cons (contents k) Seq.createEmpty
+  else cons (contents k) (init_aux len (k+1) contents)
+let rec init len contents = if len = 0 then Seq.createEmpty else init_aux len 0 contents
+
+type lbytes (n:nat) = b:bytes{length b = n}
+
+let empty_bytes : lbytes 0 = Seq.createEmpty
+
+
+#set-options "--max_fuel 1 --max_ifuel 1 --detail_errors"
+val abyte: byte -> Tot (lbytes 1)
+let abyte b = Seq.create 1 b
+
+let abyte2 (b:byte*byte) : Tot (lbytes 2) =
+  Seq.init 2 (fun i -> if i = 0 then fst b else snd b)
+
+let get (b:bytes) (pos:nat{pos < length b}) : Tot byte = Seq.index b pos
+
+val append: b1:bytes -> b2:bytes -> Tot (b:bytes{length b = length b1 + length b2})
+let append (b1:bytes) (b2:bytes) = Seq.append b1 b2
+
+val lemma_append_empty: b:bytes -> Lemma
+  (ensures (append b empty_bytes = b))
+
+let rec lemma_append_empty (b:bytes) =
+  Seq.append_empty_r b
+
+val sub: b:bytes -> s:nat{s < length b} -> e:nat{e < length b /\ s <= e} ->
+  Tot (sub:bytes)
+let sub b s e = Seq.slice b s e
+
+let lemma_sub_length (b:bytes) (s:nat{s < length b})
+  (e:nat{e < length b /\ s <= e})
+  : Lemma (length (sub b s e) = e - s)
+  = lemma_len_slice b s e
+
+assume val make: len:nat -> f:(n:nat{n < len} -> Tot byte) -> Tot (lbytes len)
+assume val create: len:nat -> Tot (lbytes len)
+assume val utf8_encode: string -> bytes
+assume val utf8_decode: bytes -> option string
+
+type uint_t (k:nat) = n:nat{n < pow2 FStar.Mul.(8 * k)}
+
+#reset-options ""
+(* Big endian integer value of a sequence of bytes *)
+val decode_big_endian: b:bytes -> Tot (uint_t (length b)) (decreases (length b))
+let rec decode_big_endian b =
+  let open FStar.Mul in
+  if length b = 0 then 0
+  else UInt8.v (last b) + pow2 8 * decode_big_endian (Seq.slice b 0 (length b - 1))
+
+val decode_big_endian_acc: b:bytes -> k:nat -> acc:uint_t k ->
+  Tot (uint_t (k + length b)) (decreases (length b))
+
+let rec decode_big_endian_acc b k acc =
+  let open FStar.Mul in
+    if length b = 0 then acc
+    else
+      let acc2 = UInt8.v (last b) + 256 * acc in
+      FStar.Math.Lemmas.pow2_plus 8 (8 * k);
+      //assert(255 + 256 * acc < pow2 (8 * (k + 1)));
+      assert(UInt8.v (last b) + 256 * acc < pow2 (8 * (k+1)));
+      //assert(acc2 < pow2 8 + pow2 (8 * (k+1)));
+      decode_big_endian_acc (slice b 0 (length b - 1)) (k + 1) acc2
+
+val eq_lemma_decode_big_endion: b:bytes ->
+  Lemma (decode_big_endian b = decode_big_endian_acc b 0 0)
+
+//let rec eq_lemma b =
+//  if length b = 0 then unit
+//  else eq_lemma (tail b)
+
+
+
+
+// TODO only use abstract functions on bytes rather than Seq functions
+
+(* Little endian integer value of a sequence of bytes *)
+val decode_little_endian: b:bytes ->
+  Tot (uint_t (length b)) (decreases (length b))
+let rec decode_little_endian b =
+  let open FStar.Mul in
+  if length b = 0 then 0
+  else UInt8.v (head b) + pow2 8 * decode_little_endian (tail b)
+
+val decode_little_endian_acc: b:bytes -> k:nat -> acc:uint_t k ->
+    Tot (uint_t (k + length b)) (decreases (length b))
+
+let rec decode_little_endian_acc b k acc =
+  let open FStar.Mul in
+    if length b = 0 then acc
+    else
+      let acc2 = UInt8.v (head b) + 256 * acc in
+        FStar.Math.Lemmas.pow2_plus 8 (8 * k);
+        assert(UInt8.v (last b) + 256 * acc < pow2 (8 * (k+1)));
+        decode_little_endian_acc (tail b) (k + 1) acc2
+
+val eq_lemma_decode_little_endian: b:bytes ->
+  Lemma (decode_little_endian b = decode_little_endian_acc b 0 0)
+
+val slice: b:bytes -> i:nat -> j:nat{i <= j && j <= length b} ->
+  Tot (bytes) (decreases (length b))
+let rec slice b i j =
+  if i > 0 then slice (tail b) (i - 1) (j - 1)
+  else
+    if j = 0 then Seq.createEmpty
+    else cons (head b) (slice (tail b) i (j - 1))
+
+
+val eq_lemma_decode_big_endion:
+  b:bytes ->
+  Lemma (decode_big_endian b = decode_big_endian_acc b 0 0)
+  (decreases (lengtjh ))
+let rec eq_lemma_decode_big_endion b =
+  if length b = 0 then ()
+  //else eq_lemma_decode_big_endion (tail b)
+  else
+    let sub = slice b 0 (length b - 1) in
+    assert(length sub = length b - 1);
+    eq_lemma_decode_big_endion sub
+
+(*
+val eq_lemma_decode_big_endion: b:bytes ->
+  GTot (u:unit{decode_big_endian b = decode_big_endian_acc b 0 0})
+  (decreases (length b))
+*)
+(*
+val eq_lemma_decode_big_endian: b:bytes ->
+  Lemma (decode_big_endian b = decode_big_endian_acc b 0 0)
+
+let rec eq_lemma_decode_big_endion b =
+  if length b = 0 then ()
+  else eq_lemma_decode_big_endion (tail b)
+  //else eq_lemma_decode_big_endion (slice b 0 (length b - 1))
+*)
+
+
+
+
+(* code transfered from Platform.Bytes.fst *)
+
+val seq_of_bytes: b:bytes -> GTot (bytes)
+let seq_of_bytes b = b
+
+val op_At_Bar: bytes -> bytes -> Tot bytes
+let op_At_Bar (b1:bytes) (b2:bytes) = append b1 b2
+
+(*@ type (l:nat) lbytes = (b:bytes){Length (b) = l} @*)
+type lbytes (l:nat) = b:bytes{length b = l}
+
+(*@ val empty_bytes : (b:bytes){B (b) = C_array_of_list C_op_Nil ()} @*)
+val empty_bytes : lbytes 0
+let empty_bytes = Seq.createEmpty
+
+val abyte : (byte -> Tot bytes)
+let abyte (b:byte) = create 1 b
+
+val abyte2 : (byte * byte) -> Tot bytes
+let abyte2 (b1, b2) = append (Seq.create 1 b1) (Seq.create 1 b2)
+
+val createBytes : l:nat -> byte -> Tot (lbytes l)
+let createBytes l b = Seq.create l b
+
+val initBytes: l:nat -> (i:nat {i<l} -> Tot byte) -> Tot (lbytes l)
+let initBytes l f = Seq.init l f
+
+(*@ assume val equalBytes : (b0:bytes -> (b1:bytes -> (r:bool){r = True /\ B (b0) = B (b1) \/ r = False /\ B (b0) <> B (b1)})) @*)
+assume val equalBytes : b1:bytes -> b2:bytes -> Tot (b:bool{b = (b1=b2)})
+(*@ assume val xor : (bytes -> (bytes -> (nb:nat -> (b3:bytes){Length (b3) = nb}))) @*)
+
+assume val xor: l:nat -> lbytes l -> lbytes l -> Tot (lbytes l)
+
+val split: b:bytes -> n:nat{n <= length b} ->
+  Tot (x:(bytes * bytes) {length (fst (x)) = n
+    /\ length (snd (x)) == (length b) - n }) //(lbytes n * lbytes (length b - n))
+
+let split b (n:nat { n <= length b}) = Seq.split b n
+
+val lemma_split : s:bytes -> i:nat{(0 <= i /\ i <= length s)} -> Lemma
+  (ensures ((fst (split s i)) @| (snd (split s i)) = s))
+let lemma_split s i =
+  cut (Seq.equal ((fst (split s i)) @| (snd (split s i)))  s)
+
+val split_eq: s:bytes -> i:nat{(0 <= i /\ i <= length s)} -> Pure
+  (x:(bytes * bytes){length (fst x) = i && length (snd x) = length s - i})
+  (requires True)
+  (ensures (fun x -> ((fst x) @| (snd x) = s)))
+let split_eq s i =
+  let x = split s i in
+  lemma_split s i;
+  x
+
+val lemma_append_inj: s1:bytes -> s2:bytes -> t1:bytes -> t2:bytes {length s1 = length t1 \/ length s2 = length t2} ->
+  Lemma (requires (Seq.equal (append s1 s2) (append t1 t2)))
+        (ensures (Seq.equal s1 t1 /\ Seq.equal s2 t2))
+let lemma_append_inj s1 s2 t1 t2 = admit()
+
+let append_empty_bytes_l (l: bytes): Lemma (ensures (empty_bytes @| l == l)) =
+  Seq.append_empty_l l
+
+let append_empty_bytes_r (l: bytes): Lemma (ensures (l @| empty_bytes == l)) =
+  Seq.append_empty_r l
+
+let append_assoc (l1 l2 l3: bytes): Lemma
+  (ensures ((l1 @| l2) @| l3 == l1 @| (l2 @| l3))) =
+  Seq.append_assoc l1 l2 l3
+
+
+
+#reset-options "--initial_fuel 1 --max_fuel 1"
+
+val encode_big_endian: k:nat -> n:uint_t k ->
+  Tot (b:lbytes k {n = decode_big_endian b}) (decreases k)
+
+// TODO
+
+// turns an integer into a bytestream, little-endian
+val encode_little_endian: k:nat -> n:uint_t k ->
+ Tot (b:lbytes k {n == decode_little_endian b}) (decreases k)
+let rec little_bytes len n =
+ if len = 0ul then
+   Seq.createEmpty
+ else
+   let len = len -^ 1ul in
+   let byte = UInt8.uint_to_t (n % 256) in
+   let n' = n / 256 in
+//   Math.Lemmas.pow2_plus 8 (8 * v len);
+   assert(n' < pow2 (8 * v len ));
+   let b' = little_bytes len n' in
+   let b = cons byte b' in
+   assert(Seq.equal b' (tail b));
+   b
+
+#reset-options "--initial_fuel 1 --max_fuel 1"
+val little_endian_null: len:nat{len < 16} -> Lemma
+ (little_endian (Seq.create len 0uy) == 0)
+
+val little_endian_singleton: n:UInt8.t -> Lemma
+ (little_endian (Seq.create 1 n) == UInt8.v n)
+
+#reset-options "--initial_fuel 1 --max_fuel 1 --z3rlimit 50"
+
+val little_endian_append: w1:bytes -> w2:bytes -> Lemma
+ (requires True)
+ (ensures
+   little_endian (Seq.append w1 w2) ==
+   little_endian w1 + pow2 (8 * Seq.length w1) * little_endian w2)
+ (decreases (Seq.length w1))
